feat: generalize split predicates

src/DY.Lib.SplitPredicate.fst
@@ -16,52 +16,64 @@ noeq type split_predicate_input_values = {
     (requires encode_label l1 == encode_label l2)
     (ensures l1 == l2)
   ;
+
+  local_pred:Type;
+  global_pred:Type;
+  apply_local_pred: local_pred -> raw_data_t -> prop;
+  apply_global_pred: global_pred -> labeled_data_t -> prop;
+  mk_global_pred: (labeled_data_t -> prop) -> global_pred;
+  apply_mk_global_pred: bare:(labeled_data_t -> prop) -> x:labeled_data_t -> Lemma
+    (apply_global_pred (mk_global_pred bare) x == bare x)
 }
 
 // Can probably be generalized to handle kdf usage too?
-type global_pred (func:split_predicate_input_values) =
+type bare_global_pred (func:split_predicate_input_values) =
   func.labeled_data_t -> prop
-type local_pred (func:split_predicate_input_values) =
+type bare_local_pred (func:split_predicate_input_values) =
   func.raw_data_t -> prop
 
-val has_local_pred: func:split_predicate_input_values -> global_pred func -> func.label_t -> local_pred func -> prop
+val has_local_pred: func:split_predicate_input_values -> func.global_pred -> func.label_t -> func.local_pred -> prop
 let has_local_pred func gpred the_label lpred =
   forall labeled_data.
     match func.decode_labeled_data labeled_data with
     | Some (label, raw_data) ->
-      label == func.encode_label the_label ==> (gpred labeled_data <==> lpred raw_data)
+      label == func.encode_label the_label ==> (func.apply_global_pred gpred labeled_data <==> func.apply_local_pred lpred raw_data)
     | None -> True
 
-val mk_global_pred: func:split_predicate_input_values -> list (func.label_t & local_pred func) -> global_pred func
-let rec mk_global_pred func l labeled_data =
+val mk_global_pred_aux: func:split_predicate_input_values -> list (func.label_t & func.local_pred) -> bare_global_pred func
+let rec mk_global_pred_aux func l labeled_data =
   match l with
   | [] -> False
   | (the_label, lpred)::t ->
     let cur_prop =
       match func.decode_labeled_data labeled_data with
       | Some (label, raw_data) ->
-        label == func.encode_label the_label /\ lpred raw_data
+        label == func.encode_label the_label /\ func.apply_local_pred lpred raw_data
       | None -> False
     in
-    cur_prop \/ mk_global_pred func t labeled_data
+    cur_prop \/ mk_global_pred_aux func t labeled_data
 
-val mk_global_pred_wrong_label:
+val mk_global_pred: func:split_predicate_input_values -> list (func.label_t & func.local_pred) -> func.global_pred
+let mk_global_pred func l =
+  func.mk_global_pred (mk_global_pred_aux func l)
+
+val mk_global_pred_aux_wrong_label:
   func:split_predicate_input_values ->
-  the_label:func.label_t -> l:list (func.label_t & local_pred func) -> labeled_data:func.labeled_data_t ->
+  the_label:func.label_t -> l:list (func.label_t & func.local_pred) -> labeled_data:func.labeled_data_t ->
   Lemma
   (requires ~(List.Tot.memP the_label (List.Tot.map fst l)))
   (ensures (
     match func.decode_labeled_data labeled_data with
     | Some (label, raw_data) ->
-      label == func.encode_label the_label ==> ~(mk_global_pred func l labeled_data)
-    | None -> ~(mk_global_pred func l labeled_data)
+      label == func.encode_label the_label ==> ~(mk_global_pred_aux func l labeled_data)
+    | None -> ~(mk_global_pred_aux func l labeled_data)
   ))
-let rec mk_global_pred_wrong_label func the_label l labeled_data =
+let rec mk_global_pred_aux_wrong_label func the_label l labeled_data =
   match l with
   | [] -> ()
   | (label, _)::t -> (
     FStar.Classical.move_requires_2 func.encode_label_inj the_label label;
-    mk_global_pred_wrong_label func the_label t labeled_data
+    mk_global_pred_aux_wrong_label func the_label t labeled_data
   )
 
 val disjointP: #a:Type -> list a -> list a -> prop
@@ -96,37 +108,38 @@ let rec memP_map #a #b f l x =
     with _. memP_map f t x
 
 val mk_global_pred_correct_aux:
-  func:split_predicate_input_values -> gpred:global_pred func -> lpreds1:list (func.label_t & local_pred func) -> lpreds2:list (func.label_t & local_pred func) -> the_label:func.label_t -> lpred:local_pred func ->
+  func:split_predicate_input_values -> gpred:bare_global_pred func -> lpreds1:list (func.label_t & func.local_pred) -> lpreds2:list (func.label_t & func.local_pred) -> the_label:func.label_t -> lpred:func.local_pred ->
   Lemma
   (requires
-    (forall labeled_data. (mk_global_pred func lpreds1 labeled_data \/ mk_global_pred func lpreds2 labeled_data) <==> gpred labeled_data) /\
+    (forall labeled_data. (mk_global_pred_aux func lpreds1 labeled_data \/ mk_global_pred_aux func lpreds2 labeled_data) <==> gpred labeled_data) /\
     List.Tot.no_repeats_p (List.Tot.map fst lpreds1) /\
     disjointP (List.Tot.map fst lpreds1) (List.Tot.map fst lpreds2) /\
     List.Tot.memP (the_label, lpred) lpreds1
   )
-  (ensures has_local_pred func gpred the_label lpred)
+  (ensures has_local_pred func (func.mk_global_pred gpred) the_label lpred)
 let rec mk_global_pred_correct_aux func gpred lpreds1 lpreds2 the_label lpred =
   match lpreds1 with
   | [] -> ()
   | (h_lab, h_spred)::t -> (
-    eliminate h_lab == the_label \/ h_lab =!= the_label returns _ with _. (
+    eliminate h_lab == the_label \/ h_lab =!= the_label returns has_local_pred func (func.mk_global_pred gpred) the_label lpred with _. (
       introduce forall labeled_data. (
         match func.decode_labeled_data labeled_data with
         | Some (label, raw_data) ->
-          label == func.encode_label the_label ==> (gpred labeled_data <==> lpred raw_data)
+          label == func.encode_label the_label ==> (gpred labeled_data <==> func.apply_local_pred lpred raw_data)
         | None -> True
       ) with (
         match func.decode_labeled_data labeled_data with
         | Some (label, raw_data) -> (
           eliminate label == func.encode_label the_label \/ label =!= func.encode_label the_label returns _ with _. (
             func.encode_label_inj the_label h_lab;
-            mk_global_pred_wrong_label func the_label t labeled_data;
-            mk_global_pred_wrong_label func the_label lpreds2 labeled_data;
+            mk_global_pred_aux_wrong_label func the_label t labeled_data;
+            mk_global_pred_aux_wrong_label func the_label lpreds2 labeled_data;
             FStar.Classical.move_requires_3 memP_map fst t (the_label, lpred)
           ) and _. ()
         )
         | None -> ()
-      )
+      );
+      FStar.Classical.forall_intro (func.apply_mk_global_pred gpred)
     ) and _. (
       disjointP_cons h_lab (List.Tot.map fst t) (List.Tot.map fst lpreds2);
       mk_global_pred_correct_aux func gpred t ((h_lab, h_spred)::lpreds2) the_label lpred
@@ -140,7 +153,7 @@ let rec disjointP_nil #a l =
   | _::t -> disjointP_nil t
 
 val mk_global_pred_correct:
-  func:split_predicate_input_values -> lpreds:list (func.label_t & local_pred func) -> the_label:func.label_t -> lpred:local_pred func ->
+  func:split_predicate_input_values -> lpreds:list (func.label_t & func.local_pred) -> the_label:func.label_t -> lpred:func.local_pred ->
   Lemma
   (requires
     List.Tot.no_repeats_p (List.Tot.map fst lpreds) /\
@@ -149,24 +162,51 @@ val mk_global_pred_correct:
   (ensures has_local_pred func (mk_global_pred func lpreds) the_label lpred)
 let mk_global_pred_correct func lpreds the_label lpred =
   disjointP_nil (List.Tot.map fst lpreds);
-  mk_global_pred_correct_aux func (mk_global_pred func lpreds) lpreds [] the_label lpred
+  mk_global_pred_correct_aux func (mk_global_pred_aux func lpreds) lpreds [] the_label lpred
 
-val mk_global_pred_eq:
-  func:split_predicate_input_values -> lpreds:list (func.label_t & local_pred func) ->
+val mk_global_pred_eq_aux:
+  func:split_predicate_input_values -> lpreds:list (func.label_t & func.local_pred) ->
   labeled_data:func.labeled_data_t ->
   Lemma
-  (mk_global_pred func lpreds labeled_data <==> (
+  ((mk_global_pred_aux func lpreds) labeled_data <==> (
       exists lab lpred raw_data.
         List.Tot.memP (lab, lpred) lpreds /\
-        lpred raw_data /\
+        func.apply_local_pred lpred raw_data /\
         func.decode_labeled_data labeled_data == Some (func.encode_label lab, raw_data)
     )
   )
-let rec mk_global_pred_eq func lpreds labeled_data =
+let rec mk_global_pred_eq_aux func lpreds labeled_data =
   match lpreds with
   | [] -> ()
   | (the_label, lpred)::tpreds ->
-    mk_global_pred_eq func tpreds labeled_data;
+    mk_global_pred_eq_aux func tpreds labeled_data;
     match func.decode_labeled_data labeled_data with
     | None -> ()
     | Some (label, raw_data) -> ()
+
+val mk_global_pred_eq:
+  func:split_predicate_input_values -> lpreds:list (func.label_t & func.local_pred) ->
+  labeled_data:func.labeled_data_t ->
+  Lemma
+  (func.apply_global_pred (mk_global_pred func lpreds) labeled_data <==> (
+      exists lab lpred raw_data.
+        List.Tot.memP (lab, lpred) lpreds /\
+        func.apply_local_pred lpred raw_data /\
+        func.decode_labeled_data labeled_data == Some (func.encode_label lab, raw_data)
+    )
+  )
+let mk_global_pred_eq func lpreds labeled_data =
+  func.apply_mk_global_pred (mk_global_pred_aux func lpreds) labeled_data;
+  mk_global_pred_eq_aux func lpreds labeled_data
+
+val local_eq_global_lemma:
+  func:split_predicate_input_values ->
+  gpred:func.global_pred -> the_label:func.label_t -> lpred:func.local_pred ->
+  labeled_data:func.labeled_data_t -> raw_data:func.raw_data_t ->
+  Lemma
+  (requires
+    func.decode_labeled_data labeled_data == Some (func.encode_label the_label, raw_data) /\
+    has_local_pred func gpred the_label lpred
+  )
+  (ensures func.apply_global_pred gpred labeled_data <==> func.apply_local_pred lpred raw_data)
+let local_eq_global_lemma func gpred the_label lpred labeled_data raw_data = ()
